src/coq/CFG.v
@@ -37,7 +37,7 @@ Section hiding_notations.
   Global Instance show_pc : Show pc :=
     { show p := "@" << show (fn p) << ":" << show (bk p) << ":" << show (pt p)}.
 End hiding_notations.
-  
+
 
 Ltac unfold_eqv :=
   repeat (unfold eqv in *; unfold eqv_raw_id in *; unfold eqv_instr_id in *).
@@ -63,7 +63,7 @@ Module PC <: UsualDecidableTypeFull.
   Defined.
 
   Include HasEqDec2Bool.
-  
+
 End PC.
 Instance eq_dec_pc : RelDec (@eq pc) := RelDec_from_dec (@eq pc) PC.eq_dec.
 
@@ -72,24 +72,24 @@ Instance eq_dec_pc : RelDec (@eq pc) := RelDec_from_dec (@eq pc) PC.eq_dec.
 Section CFG.
   Variable (T:Set).
 
-(* TODO: rename Step to Inst *)
-Inductive cmd : Set :=
-| Inst (i:instr T) 
-| Term (t:terminator T)
-.                    
+  (* TODO: rename Step to Inst *)
+  Inductive cmd : Set :=
+  | Inst (i:instr T)
+  | Term (t:terminator T)
+  .
 
 
-(* each function definition corresponds to a control-flow graph 
+  (* each function definition corresponds to a control-flow graph
    - init is the entry block
    - blks is a list of labeled blocks
    - args is the list of identifiers brought into scope by this function
-*)
-Record cfg := mkCFG
-{
-  init : block_id;
-  blks : list (block T);
-  args : list ident;
-}.
+   *)
+  Record cfg := mkCFG
+                  {
+                    init : block_id;
+                    blks : list (block T);
+                    args : list ident;
+                  }.
 
 (* An mcfg is a module where each function body has been converted to a cfg *)
 Definition mcfg : Set := modul T cfg.
@@ -98,7 +98,7 @@ Definition find_defn {X:Set} (fid:function_id) (d:definition T X) : option (defi
   if (ident_of d) ~=? (ID_Global fid) then Some d else None.
 
 Definition find_function (CFG : mcfg) (fid:function_id) : option (definition T cfg) :=
-  find_map (find_defn fid) (m_definitions T _ CFG).
+  find_map (find_defn fid) (m_definitions CFG).
 
 
 Definition fallthrough (cd: (code T)) term_id : instr_id :=
@@ -107,19 +107,19 @@ Definition fallthrough (cd: (code T)) term_id : instr_id :=
   | (next, _)::_ => next
   end.
 
-Definition blk_term_id b := fst (blk_term T b).
-Definition blk_terminator b := snd (blk_term T b).
+Definition blk_term_id (b: block T) := fst (blk_term b).
+Definition blk_terminator (b: block T) := snd (blk_term b).
 
-Definition blk_entry_id (b:block T) : instr_id := fallthrough (blk_code T b) (blk_term_id b). 
+Definition blk_entry_id (b:block T) : instr_id := fallthrough (blk_code b) (blk_term_id b).
 
 Definition blk_entry_pc (fid:function_id) (b:block T) :=
-  mk_pc fid (blk_id T b) (blk_entry_id b).
+  mk_pc fid (blk_id b) (blk_entry_id b).
 
 Definition blk_term_pc (fid:function_id) (b:block T) :=
-  mk_pc fid (blk_id T b) (blk_term_id b).
+  mk_pc fid (blk_id b) (blk_term_id b).
 
 Fixpoint find_block bs block_id : option (block T) :=
-  find (fun b => if (blk_id T b) ~=? block_id then true else false) bs.
+  find (fun b => if (blk_id b) ~=? block_id then true else false) bs.
 
 Fixpoint find_instr (cd : (code T)) (p:instr_id) (t:instr_id) : option (cmd * option instr_id) :=
   match cd with
@@ -132,23 +132,23 @@ Fixpoint find_instr (cd : (code T)) (p:instr_id) (t:instr_id) : option (cmd * op
   end.
 
 Definition block_to_cmd (b:block T) (iid:instr_id) : option (cmd * option instr_id) :=
-  let term_id := blk_term_id b in 
+  let term_id := blk_term_id b in
   if term_id ~=? iid then
-    Some (Term (snd (blk_term T b)), None)
+    Some (Term (snd (blk_term b)), None)
   else
-    find_instr (blk_code T b) iid term_id 
+    find_instr (blk_code b) iid term_id
 .
 
 (*
 Definition fetch (CFG : mcfg) (p:pc) : option cmd:=
-  let 'mk_pc fid bid iid := p in 
+  let 'mk_pc fid bid iid := p in
   cfg <- find_function CFG fid ;;
   blk <- find_block (blks (df_instrs T cfg)) bid ;;
   '(c, _) <- block_to_cmd blk iid ;;
   ret c.
-   
+
 Definition incr_pc (CFG:mcfg) (p:pc) : option pc :=
-  let 'mk_pc fid bid iid := p in 
+  let 'mk_pc fid bid iid := p in
   cfg <- find_function CFG fid ;;
   blk <- find_block (blks (df_instrs T cfg)) bid ;;
   '(c, n) <- block_to_cmd blk iid ;;
@@ -160,12 +160,12 @@ Inductive block_entry : Set :=
 | BlockEntry (phis:list (local_id * (phi T))) (p:pc).
 
 Definition block_to_entry (fid:function_id) (b:block T) : block_entry :=
-  BlockEntry (blk_phis T b) (blk_entry_pc fid b).
+  BlockEntry (blk_phis b) (blk_entry_pc fid b).
 
 Definition find_block_entry (CFG:mcfg) (fid:function_id) (bid:block_id) : option block_entry :=
   cfg <- find_function CFG fid ;;
-  blk <- find_block (blks (df_instrs T _ cfg)) bid ;;
-  ret (block_to_entry fid blk).  
+  blk <- find_block (blks (df_instrs cfg)) bid ;;
+  ret (block_to_entry fid blk).
 
 Inductive function_entry : Set :=
 | FunctionEntry (args:list local_id) (p:pc).
@@ -173,15 +173,15 @@ Inductive function_entry : Set :=
 
 Definition find_function_entry (CFG:mcfg) (fid:function_id) : option function_entry :=
   dfn <- find_function CFG fid ;;
-  let cfg := df_instrs T _ dfn in
+  let cfg := df_instrs dfn in
   blk <- find_block (blks cfg) (init cfg) ;;
-  ret (FunctionEntry (df_args T _ dfn) (mk_pc fid (init cfg) (blk_entry_id blk))).  
+  ret (FunctionEntry (df_args dfn) (mk_pc fid (init cfg) (blk_entry_id blk))).
 
 
 (*
 Definition code_of_definition (d:definition (list block)) (p:pt) : option cmd :=
   cmd_from_blocks p (df_instrs d).
-  
+
 Definition blks_of_definition (d:definition (list block)) block_id : option pt :=
   'b <- lookup_block (df_instrs d) block_id;
   Some (fallthrough (blk_term_id b) (blk_instrs b)).
@@ -191,41 +191,38 @@ Definition phis_of_definition (d:definition (list block)) block_id : option bloc
   block_to_phis b.
 *)
 
-Definition init_of_definition d : option block_id :=
-  match (df_instrs T _ d) with
+Definition init_of_definition (d: definition T (list (block T))) : option block_id :=
+  match (df_instrs d) with
   | [] => None
-  | b :: _ => Some (blk_id T b)
+  | b :: _ => Some (blk_id b)
   end.
-
 
 Definition cfg_of_definition (d:definition T (list (block T))) : option cfg :=
   init <- init_of_definition d ;;
-  let args := List.map (fun x => ID_Local x) (df_args T _ d) in
+  let args := List.map (fun x => ID_Local x) (df_args d) in
     Some {| init := init;
-            blks := df_instrs T _ d;
+            blks := df_instrs d;
             args := args;
          |}.
-
 
 Definition mcfg_of_modul (m:modul T (list (block T))) : option mcfg :=
   defns <- map_option
                 (fun d =>
                    cfg <- cfg_of_definition d ;;
                      Some {|
-                       df_prototype := df_prototype T _ d;
-                       df_args := df_args T _ d;
+                       df_prototype := df_prototype d;
+                       df_args := df_args d;
                        df_instrs := cfg
-                       |}) (m_definitions T _ m) ;;
+                       |}) (m_definitions m) ;;
   Some {|
-    m_name := m_name T _ m;
-    m_target := m_target T _ m;
-    m_datalayout := m_datalayout _ _ m;
-    m_type_defs := m_type_defs _ _ m;
-    m_globals := m_globals _ _ m;
-    m_declarations := m_declarations _ _ m;
+    m_name := m_name m;
+    m_target := m_target m;
+    m_datalayout := m_datalayout m;
+    m_type_defs := m_type_defs m;
+    m_globals := m_globals m;
+    m_declarations := m_declarations m;
     m_definitions := defns
   |}.
 
 (*  ------------------------------------------------------------------------- *)
 End CFG.
-
